@prefix schema: <https://schema.org/> .
@prefix qudt:  <http://qudt.org/2.0/schema/qudt#> .
@prefix adms:  <http://www.w3.org/ns/adms#> .
@prefix owl:   <http://www.w3.org/2002/07/owl#> .
@prefix xsd:   <http://www.w3.org/2001/XMLSchema#> .
@prefix skos:  <http://www.w3.org/2004/02/skos/core#> .
@prefix rdfs:  <http://www.w3.org/2000/01/rdf-schema#> .
@prefix ofd:   <https://w3id.org/openfooddata/core#> .
@prefix vf:    <https://w3id.org/valueflows/> .
@prefix rdf:   <http://www.w3.org/1999/02/22-rdf-syntax-ns#> .
@prefix dcterms: <http://purl.org/dc/terms/> .
@prefix vann:  <http://purl.org/vocab/vann/> .
@prefix foaf:  <http://xmlns.com/foaf/0.1/> .
@prefix dc:    <http://purl.org/dc/elements/1.1/> .

ofd:broaderFoodType  a      owl:ObjectProperty ;
        rdfs:domain         ofd:FoodProduct ;
        rdfs:label          "broaderFoodType" ;
        rdfs:range          ofd:FoodType ;
        rdfs:subPropertyOf  skos:broadMatch ;
        skos:prefLabel      "food category"@en .

ofd:producesFoodType  a  owl:ObjectProperty ;
        rdfs:domain  foaf:Agent ;
        rdfs:label   "offers FoodType" ;
        rdfs:range   ofd:FoodType .

ofd:isLookingForPartners
        a            owl:DataProperty ;
        rdfs:domain  foaf:Agent ;
        rdfs:label   "isLookingForPartners" ;
        rdfs:range   xsd:boolean .

ofd:FoodType  a       owl:Class ;
        rdfs:comment  "base class for hierarchical classification of Food Types" ;
        rdfs:label    "Food Type" .

<https://w3id.org/openfooddata/core>
        a                              adms:SemanticAsset , owl:Ontology ;
        dc:creator                     ofd:Kalin ;
        dc:license                     "https://creativecommons.org/publicdomain/" ;
        dcterms:created                "2017-02-17"^^xsd:date ;
        dcterms:description            "This ontology models the Open Food Data domain. It allows to describe food products, food producers/farmers, food shops/hubs and other actors and collaboration agreements between those" ;
        dcterms:modified               "2017-04-18"^^xsd:date ;
        dcterms:partOf                 <https://w3id.org/openfooddata/> ;
        dcterms:publisher              ofd:OFD ;
        dcterms:status                 <http://purl.org/adms/status/UnderDevelopment> ;
        dcterms:title                  "Open Food Data Ontology" ;
        dcterms:type                   <http://purl.org/adms/assettype/Ontology> ;
        vann:preferredNamespacePrefix  "ofd" ;
        vann:preferredNamespaceUri     "https://w3id.org/openfooddata/core" ;
        foaf:homepage                  <https://w3id.org/openfooddata/core> .

ofd:FoodActorType  a  owl:Class ;
        rdfs:comment  "base class for hierarchical or other classification of Food Actors" ;
        rdfs:label    "Food Actor Type" .

ofd:operationalCoverage
        a             owl:ObjectProperty ;
        rdfs:comment  "activity coverage of a specific actor, which may depend on its agreements with other actors" ;
        rdfs:domain   foaf:Agent ;
        rdfs:label    "operationalCoverage" ;
        rdfs:range    schema:GeoShape .

ofd:offersProduct  a  owl:ObjectProperty ;
        rdfs:domain  foaf:Agent ;
        rdfs:label   "offers Product" ;
        rdfs:range   ofd:FoodProduct .

ofd:quantitativeRestriction
        a                   owl:ObjectProperty ;
        rdfs:comment        "custom restrictions that the Service can handle min and max or more values may be used" ;
        rdfs:domain         ofd:FoodServiceType ;
        rdfs:label          "quantitativeRestriction" ;
        rdfs:range          qudt:Value ;
        rdfs:subPropertyOf  skos:semanticRelation .

ofd:canHandleFoodType
        a                   owl:ObjectProperty ;
        rdfs:comment        "indicates that specific food taype is can be handled by this service" ;
        rdfs:domain         ofd:FoodServiceType ;
        rdfs:label          "canHandleFoodType" ;
        rdfs:range          ofd:FoodType ;
        rdfs:subPropertyOf  skos:semanticRelation .

ofd:claimedBy  a      owl:ObjectProperty ;
        rdfs:comment  "Identifies the Agent who claimed ownership on this Food Actor and its data" ;
        rdfs:domain   foaf:Agent ;
        rdfs:label    "claimedBy" ;
        rdfs:range    foaf:Agent .

ofd:canNotHandleFoodType
        a                   owl:ObjectProperty ;
        rdfs:comment        "indicates that specific food taype is cannot be handled by this service" ;
        rdfs:domain         ofd:FoodServiceType ;
        rdfs:label          "canNotHandleFoodType" ;
        rdfs:range          ofd:FoodType ;
        rdfs:subPropertyOf  skos:semanticRelation .

ofd:offersNonFoodItem
        a            owl:ObjectProperty ;
        rdfs:domain  foaf:Agent ;
        rdfs:label   "offersNonFoodItem" ;
        rdfs:range   ofd:NonFoodItem .

ofd:narrowerFoodProduct
        a                   owl:ObjectProperty ;
        rdfs:domain         ofd:FoodType ;
        rdfs:label          "narrowerFoodProduct" ;
        rdfs:range          ofd:FoodProduct ;
        rdfs:subPropertyOf  skos:narrowMatch ;
        owl:inverseOf       ofd:broaderFoodType ;
        skos:prefLabel      "related food product"@en .

ofd:offersService  a  owl:ObjectProperty ;
        rdfs:domain  foaf:Agent ;
        rdfs:label   "provides Service" ;
        rdfs:range   ofd:FoodServiceType .

ofd:actorType  a     owl:ObjectProperty ;
        rdfs:domain  foaf:Agent ;
        rdfs:label   "actor Type" ;
        rdfs:range   ofd:FoodActorType .

ofd:relatedFoodProduct
        a                   owl:ObjectProperty ;
        rdfs:comment        "relates concept to a FoodService" ;
        rdfs:domain         skos:Concept ;
        rdfs:label          "relatedFoodProduct" ;
        rdfs:range          ofd:FoodProduct ;
        rdfs:subPropertyOf  skos:semanticRelation .

ofd:producedBy  a    owl:ObjectProperty ;
        rdfs:domain  ofd:FoodProduct ;
        rdfs:label   "producedBy" ;
        rdfs:range   foaf:Agent .

ofd:harvestTime  a    owl:ObjectProperty ;
        rdfs:comment  "the min number of day/hours for the product to be available after purchase" ;
        rdfs:domain   ofd:FoodProduct ;
        rdfs:label    "harvestPeriod" ;
        rdfs:range    qudt:QuantityValue .

ofd:usedInMaking  a         owl:ObjectProperty ;
        rdfs:domain         ofd:FoodProduct ;
        rdfs:label          "usedInMaking" ;
        rdfs:range          ofd:FoodProduct ;
        rdfs:subPropertyOf  skos:semanticRelation ;
        owl:inverseOf       ofd:madeOf .

ofd:relatedFoodType  a      owl:ObjectProperty ;
        rdfs:comment        "relates concept to a FoodService" ;
        rdfs:domain         skos:Concept ;
        rdfs:label          "relatedFoodType" ;
        rdfs:range          ofd:FoodType ;
        rdfs:subPropertyOf  skos:semanticRelation .

ofd:Kalin  a           foaf:Person ;
        owl:SameAs     <http://djodjo.org#az> ;
        foaf:homepage  <http://djodjo.org> ;
        foaf:name      "Kalin Maldzhanski" .

ofd:FoodProduct  a    owl:Class ;
        rdfs:comment  "base class for Food Products. Instances are not actual Offerings. Instances might also be of type schema:Product" ;
        rdfs:label    "Food Product" .

ofd:relatedService  a       owl:ObjectProperty ;
        rdfs:comment        "relates concept to a FoodService" ;
        rdfs:domain         skos:Concept ;
        rdfs:label          "relatedService" ;
        rdfs:range          ofd:FoodServiceType ;
        rdfs:subPropertyOf  skos:semanticRelation .

ofd:OFD  a             dcterms:Agent ;
        foaf:homepage  <http://www.openfooddata.org/> ;
        foaf:member    ofd:Kalin ;
        foaf:name      "Open Food Data" .

ofd:storageTemp  a    owl:ObjectProperty ;
        rdfs:comment  "Temp range depending on the cold/heat tolerance of the food min and max or more values may be used" ;
        rdfs:domain   ofd:FoodProduct ;
        rdfs:label    "storageTemp" ;
        rdfs:range    qudt:Value .

ofd:NonFoodItem  a  owl:Class ;
        rdfs:label  "Non-Food Item" .

ofd:madeOf  a               owl:ObjectProperty ;
        rdfs:domain         ofd:FoodProduct ;
        rdfs:label          "madeOf" ;
        rdfs:range          ofd:FoodProduct ;
        rdfs:subPropertyOf  skos:semanticRelation ;
        owl:inverseOf       ofd:usedInMaking .

ofd:storageDuration  a  owl:ObjectProperty ;
        rdfs:comment  "the allowed storage before consumption min and max or more values may be used" ;
        rdfs:domain   ofd:FoodProduct ;
        rdfs:label    "storageDuration" ;
        rdfs:range    qudt:Value .

ofd:preparationTime  a  owl:ObjectProperty ;
        rdfs:comment  "the min number of day/hours for the Actor to be available after commitment" ;
        rdfs:domain   ofd:FoodActor ;
        rdfs:label    "harvestPeriod" ;
        rdfs:range    qudt:QuantityValue .

ofd:FoodService  a    owl:Class ;
        rdfs:comment  "base class for Food Services. Instances are not actual Offerings." ;
        rdfs:label    "Food Service" .
